Introduce [Reveal] primitive. Use it to improve eio/rcfd.

theories/eio/rcfd.v
@@ -58,41 +58,43 @@ Implicit Types state : rcfd_state.
 #[local] Instance rcfd_state_eq_dec : EqDecision rcfd_state :=
   ltac:(solve_decision).
 
-#[local] Definition state_to_val state :=
+#[local] Definition state_to_val cid state :=
   match state with
   | RcfdStateOpen fd =>
-      ’Open{ fd }
+      ’Open@{cid}{ fd }
   | RcfdStateClosing fn =>
       ’Closing{ fn }
   end.
-#[local] Arguments state_to_val !_ / : assert.
-#[local] Coercion state_to_val : rcfd_state >-> val.
+#[local] Arguments state_to_val _ !_ / : assert.
 
-#[local] Instance state_to_val_inj :
-  Inj (=) (=) state_to_val.
+#[local] Instance state_to_val_inj cid :
+  Inj (=) (=) (state_to_val cid).
 Proof.
   intros [] []; naive_solver.
+Qed.
+#[local] Instance state_to_val_physical cid state :
+  ValPhysical (state_to_val cid state).
+Proof.
+  destruct state; done.
 Qed.
 
 Definition rcfd_make : val :=
   λ: "fd",
-    { #0; ref ‘Open{ "fd" } }.
+    { #0; Reveal ‘Open{ "fd" } }.
 
 #[local] Definition rcfd_closed : val :=
-  λ: <>,
-    ref ‘Closing{ λ: <>, () }.
+  ’Closing{ λ: <>, () }.
 
 #[local] Definition rcfd_put : val :=
   λ: "t",
     let: "old" := Faa "t".[ops] #-1 in
     if: "old" = #1 then (
-      let: "prev" := "t".{fd} in
-      match: !"prev" with
+      match: "t".{fd} with
       | Open <> =>
           ()
-      | Closing "no_users" =>
+      | Closing "no_users" as "prev" =>
           ifnot: #0 < "t".{ops} then
-            if: Cas "t".[fd] "prev" (rcfd_closed ()) then
+            if: Cas "t".[fd] "prev" rcfd_closed then
               "no_users" ()
       end
     ).
@@ -100,7 +102,7 @@ Definition rcfd_make : val :=
 #[local] Definition rcfd_get : val :=
   λ: "t",
     Faa "t".[ops] #1 ;;
-    match: !"t".{fd} with
+    match: "t".{fd} with
     | Open "fd" =>
         ‘Some{ "fd" }
     | Closing <> =>
@@ -110,15 +112,14 @@ Definition rcfd_make : val :=
 
 Definition rcfd_close : val :=
   λ: "t",
-    let: "prev" := "t".{fd} in
-    match: !"prev" with
-    | Open "fd" =>
+    match: "t".{fd} with
+    | Open "fd" as "prev" =>
         let: "close" <> :=
           unix_close "fd"
         in
-        let: "next" := ref ‘Closing{ "close" } in
+        let: "next" := ‘Closing{ "close" } in
         if: Cas "t".[fd] "prev" "next" then (
-          if: ("t".{ops} = #0) && Cas "t".[fd] "next" (rcfd_closed ()) then (
+          if: ("t".{ops} = #0) && Cas "t".[fd] "next" rcfd_closed then (
             "close" ()
           ) else (
             ()
@@ -133,12 +134,11 @@ Definition rcfd_close : val :=
 
 Definition rcfd_remove : val :=
   λ: "t",
-    let: "prev" := "t".{fd} in
-    match: !"prev" with
-    | Open "fd" =>
+    match: "t".{fd} with
+    | Open "fd" as "prev" =>
         let: "flag" := ref #false in
         let: "chan" := spsc_latch1_create () in
-        let: "next" := ref ‘Closing{ λ: <>, spsc_latch1_signal "chan" } in
+        let: "next" := ‘Closing{ λ: <>, spsc_latch1_signal "chan" } in
         if: Cas "t".[fd] "prev" "next" then (
           spsc_latch1_wait "chan" ;;
           ‘Some{ "fd" }
@@ -162,7 +162,7 @@ Definition rcfd_use : val :=
 
 Definition rcfd_is_open : val :=
   λ: "t",
-    match: !"t".{fd} with
+    match: "t".{fd} with
     | Open <> =>
         #true
     | Closing <> =>
@@ -171,7 +171,7 @@ Definition rcfd_is_open : val :=
 
 Definition rcfd_peek : val :=
   λ: "t",
-    match: !"t".{fd} with
+    match: "t".{fd} with
     | Open "fd" =>
         ‘Some{ "fd" }
     | Closing <> =>
@@ -220,7 +220,7 @@ Section rcfd_G.
   Record rcfd_meta := {
     rcfd_meta_tokens : gname ;
     rcfd_meta_lstate : gname ;
-    rcfd_meta_open_state : location ;
+    rcfd_meta_open_state : constr_id ;
   }.
   Implicit Types γ : rcfd_meta.
 
@@ -257,15 +257,15 @@ Section rcfd_G.
     auth_mono_lb (A := leibnizO rcfd_lstate) rcfd_lstep γ.(rcfd_meta_lstate) lstate.
 
   #[local] Definition rcfd_inv_inner l γ fd chars : iProp Σ :=
-    ∃ state lstate ops l_state,
+    ∃ state lstate ops,
     l.[ops] ↦ #ops ∗
-    l.[fd] ↦ #l_state ∗ l_state ↦□ (state : val) ∗
+    l.[fd] ↦ state_to_val γ.(rcfd_meta_open_state) state ∗
     rcfd_lstate_auth γ lstate ∗
     match lstate with
     | RcfdLstateOpen =>
         ∃ q qs,
         ⌜ops = size qs ∧ set_fold Qp.add q qs = 1%Qp⌝ ∗
-        ⌜l_state = γ.(rcfd_meta_open_state) ∧ state = RcfdStateOpen fd⌝ ∗
+        ⌜state = RcfdStateOpen fd⌝ ∗
         rcfd_tokens_auth γ qs ∗
         unix_fd_model fd (DfracOwn q) chars
     | RcfdLstateClosingUsers =>
@@ -426,18 +426,18 @@ Section rcfd_G.
   Proof.
     iIntros "%Φ Hmodel HΦ".
     wp_rec.
-    wp_alloc l_state as "Hstate". iMod (pointsto_persist with "Hstate") as "Hstate".
+    wp_reveal cid.
     wp_record l as "Hmeta" "(Hops & Hfd & _)".
     iMod rcfd_tokens_alloc as "(%γ_tokens & Htokens_auth)".
     iMod rcfd_lstate_alloc as "(%γ_lstate & Hlstate_auth)".
     pose γ := {|
       rcfd_meta_tokens := γ_tokens ;
       rcfd_meta_lstate := γ_lstate ;
-      rcfd_meta_open_state := l_state ;
+      rcfd_meta_open_state := cid ;
     |}.
     iMod (meta_set _ _ γ with "Hmeta") as "Hmeta"; first done.
     iApply "HΦ". iExists l, γ. iStep 2.
-    iApply inv_alloc. iExists (RcfdStateOpen fd). iStep 5. iExists 1%Qp, ∅. iSteps.
+    iApply inv_alloc. iExists (RcfdStateOpen fd). iStep 4. iExists 1%Qp, ∅. iSteps.
   Qed.
 
   #[local] Lemma rcfd_put_spec' l γ fd chars :
@@ -460,14 +460,14 @@ Section rcfd_G.
     wp_rec. wp_pures.
 
     wp_bind (Faa _ _).
-    iInv "Hinv" as "(%state1 & %lstate1 & %ops1 & %l_state1 & Hops & Hfd & Hstate1 & Hlstate_auth & Hlstate1)".
+    iInv "Hinv" as "(%state1 & %lstate1 & %ops1 & Hops & Hfd & Hlstate_auth & Hlstate1)".
     wp_faa.
     iSplitR "HΦ".
     { iDestruct "H" as "[(%q & Htokens_frag & Hmodel) | #Hlstate_lb]".
       - destruct lstate1.
-        + iDestruct "Hlstate1" as "(%q' & %qs & (-> & %Hqs) & (-> & ->) & Htokens_auth & Hmodel')".
+        + iDestruct "Hlstate1" as "(%q' & %qs & (-> & %Hqs) & -> & Htokens_auth & Hmodel')".
           iDestruct (rcfd_tokens_elem_of with "Htokens_auth Htokens_frag") as %Hq.
-          iExists (RcfdStateOpen _). iStep 4. iExists (q + q')%Qp, (qs ∖ {[+q+]}).
+          iExists (RcfdStateOpen _). iStep 3. iExists (q + q')%Qp, (qs ∖ {[+q+]}).
           iSplitR; [iSplitR; iPureIntro | iSplitR; [| iSplitR "Hmodel Hmodel'"]].
           * assert (qs ≠ ∅) as Hqs_size%gmultiset_size_non_empty_iff by multiset_solver.
             rewrite gmultiset_size_difference; first multiset_solver.
@@ -485,31 +485,31 @@ Section rcfd_G.
             rewrite gmultiset_difference_diag.
             iMod (rcfd_lstate_update RcfdLstateClosingNoUsers with "Hlstate_auth") as "Hlstate_auth"; first done.
             iCombine "Hmodel Hmodel'" as "Hmodel". rewrite Hqs. iDestruct ("Hfn1" with "Hmodel") as "Hfn1".
-            iExists (RcfdStateClosing _). iStep 5. done.
+            iExists (RcfdStateClosing _). iStep 4. done.
           * iMod (rcfd_tokens_update_dealloc with "Htokens_auth Htokens_frag") as "Htokens_auth".
             iCombine "Hmodel Hmodel'" as "Hmodel".
-            iExists (RcfdStateClosing _). iStep 4. iExists (q + q')%Qp, (qs ∖ {[+q+]}). iSteps; iPureIntro.
+            iExists (RcfdStateClosing _). iStep 3. iExists (q + q')%Qp, (qs ∖ {[+q+]}). iSteps; iPureIntro.
             -- rewrite gmultiset_size_difference; first multiset_solver.
                rewrite gmultiset_size_singleton. lia.
             -- rewrite gmultiset_size_difference; first multiset_solver.
                rewrite gmultiset_size_singleton. lia.
             -- rewrite (gmultiset_disj_union_difference' q qs) // gmultiset_set_fold_disj_union gmultiset_set_fold_singleton // in Hqs.
         + iDestruct "Hlstate1" as "(%fn1 & -> & Hfn1)".
-          iExists (RcfdStateClosing _). iStep 5. done.
+          iExists (RcfdStateClosing _). iStep 4. done.
       - iDestruct (rcfd_lstate_valid_closing_no_users with "Hlstate_auth Hlstate_lb") as %->.
         iDestruct "Hlstate1" as "(%fn1 & -> & Hfn1)".
-        iExists (RcfdStateClosing _). iStep 5. done.
+        iExists (RcfdStateClosing _). iStep 4. done.
     }
     iModIntro. clear.
 
     wp_pures. destruct (decide (ops1 = 1)) as [-> | Hops]; wp_pures; last iSteps.
 
     wp_bind (!_)%E.
-    iInv "Hinv" as "(%state2 & %lstate2 & %ops2 & %l_state2 & Hops & Hfd & #Hstate2 & Hlstate_auth & Hlstate2)".
+    iInv "Hinv" as "(%state2 & %lstate2 & %ops2 & Hops & Hfd & Hlstate_auth & Hlstate2)".
     wp_load.
     destruct (decide (lstate2 = RcfdLstateOpen)) as [-> | Hlstate2].
 
-    - iDestruct "Hlstate2" as "(%q & %qs & (-> & %Hqs) & (-> & ->) & Htokens_auth & Hmodel)".
+    - iDestruct "Hlstate2" as "(%q & %qs & (-> & %Hqs) & -> & Htokens_auth & Hmodel)".
       iSplitR "HΦ". { iExists (RcfdStateOpen _). iSteps. }
       iSteps.
 
@@ -526,10 +526,10 @@ Section rcfd_G.
       iSplitR "HΦ". { iExists (RcfdStateClosing _). iSteps. }
       iModIntro. clear.
 
-      wp_load. wp_pures.
+      wp_pures.
 
       wp_bind (!_)%E.
-      iInv "Hinv" as "(%state3 & %lstate3 & %ops3 & %l_state3 & Hops & Hfd & #Hstate3 & Hlstate_auth & Hlstate3)".
+      iInv "Hinv" as "(%state3 & %lstate3 & %ops3 & Hops & Hfd & Hlstate_auth & Hlstate3)".
       wp_load.
       iDestruct (rcfd_lstate_valid_closing_users with "Hlstate_auth Hlstate_lb") as %[-> | ->].
 
@@ -543,19 +543,17 @@ Section rcfd_G.
 
       + iDestruct "Hlstate3" as "(%fn3 & -> & Hfn3)".
         iClear "Hlstate_lb". iDestruct (rcfd_lstate_lb_get with "Hlstate_auth") as "#Hlstate_lb".
-        iSplitR "HΦ". { iExists (RcfdStateClosing _). iStep 5. done. }
+        iSplitR "HΦ". { iExists (RcfdStateClosing _). iStep 4. done. }
         iModIntro. clear.
 
         wp_pures. case_bool_decide as Hops3; wp_pures; first iSteps.
 
-        wp_rec. wp_alloc closed as "Hclosed". wp_pures.
-
         wp_bind (Cas _ _ _).
-        iInv "Hinv" as "(%state4 & %lstate4 & %ops4 & %l_state4 & Hops & Hfd & #Hstate4 & Hlstate_auth & Hlstate4)".
-        wp_cas as Hcas | [= <-]; first iSteps.
+        iInv "Hinv" as "(%state4 & %lstate4 & %ops4 & Hops & Hfd & Hlstate_auth & Hlstate4)".
+        wp_cas as Hcas | Hcas _; first iSteps.
+        destruct state4; first naive_solver. destruct Hcas as (_ & [= <-]).
         iDestruct (rcfd_lstate_valid_closing_no_users with "Hlstate_auth Hlstate_lb") as %->.
-        iDestruct "Hlstate4" as "(%fn4 & -> & Hfn4)".
-        iDestruct (pointsto_agree with "Hstate2 Hstate4") as %[= <-]%(inj _).
+        iDestruct "Hlstate4" as (fn4 [= <-]) "Hfn4".
         iSplitR "Hfn4 HΦ". { iExists (RcfdStateClosing _). iSteps. }
         iSteps.
   Qed.
@@ -599,7 +597,7 @@ Section rcfd_G.
     wp_rec. wp_pures.
 
     wp_bind (Faa _ _).
-    iInv "Hinv" as "(%state1 & %lstate1 & %ops1 & %l_state1 & Hops & Hfd & Hstate1 & Hlstate_auth & Hlstate1)".
+    iInv "Hinv" as "(%state1 & %lstate1 & %ops1 & Hops & Hfd & Hlstate_auth & Hlstate1)".
     wp_faa.
     iAssert (|==>
       rcfd_inv_inner l γ fd chars ∗
@@ -611,18 +609,18 @@ Section rcfd_G.
       )
     )%I with "[- HΦ]" as ">($ & H)".
     { destruct lstate1.
-      - iDestruct "Hlstate1" as "(%q & %qs & (-> & %Hqs) & (-> & ->) & Htokens_auth & Hmodel)".
+      - iDestruct "Hlstate1" as "(%q & %qs & (-> & %Hqs) & -> & Htokens_auth & Hmodel)".
         iMod (rcfd_tokens_update_alloc (q / 2) with "Htokens_auth") as "(Htokens_auth & Htokens_frag)".
         iDestruct "Hmodel" as "(Hmodel1 & Hmodel2)".
         iSplitR "Htokens_frag Hmodel2"; last iSteps.
-        iExists (RcfdStateOpen _). iStep 4. iExists (q / 2)%Qp, (qs ⊎ {[+q / 2+]})%Qp. iSteps; iPureIntro.
+        iExists (RcfdStateOpen _). iStep 3. iExists (q / 2)%Qp, (qs ⊎ {[+q / 2+]})%Qp. iSteps; iPureIntro.
         + rewrite gmultiset_size_disj_union gmultiset_size_singleton. lia.
         + rewrite (comm (⊎)) gmultiset_set_fold_disj_union gmultiset_set_fold_singleton Qp.div_2 //.
       - iDestruct "Hlstate1" as "(%q & %qs & %fn1 & (-> & %Hqs_size & %Hqs) & -> & Htokens_auth & Hmodel & Hfn1)".
         iMod (rcfd_tokens_update_alloc (q / 2) with "Htokens_auth") as "(Htokens_auth & Htokens_frag)".
         iDestruct "Hmodel" as "(Hmodel1 & Hmodel2)".
         iSplitR "Htokens_frag Hmodel2"; last iSteps.
-        iExists (RcfdStateClosing _). iStep 4. iExists (q / 2)%Qp, (qs ⊎ {[+q / 2+]})%Qp. iSteps; iPureIntro.
+        iExists (RcfdStateClosing _). iStep 3. iExists (q / 2)%Qp, (qs ⊎ {[+q / 2+]})%Qp. iSteps; iPureIntro.
         + rewrite gmultiset_size_disj_union gmultiset_size_singleton. lia.
         + rewrite gmultiset_size_disj_union. lia.
         + rewrite (comm (⊎)) gmultiset_set_fold_disj_union gmultiset_set_fold_singleton Qp.div_2 //.
@@ -634,11 +632,11 @@ Section rcfd_G.
     iModIntro. wp_pures. clear.
 
     wp_bind (!#l.[fd])%E.
-    iInv "Hinv" as "(%state2 & %lstate2 & %ops2 & %l_state2 & Hops & Hfd & #Hstate2 & Hlstate_auth & Hlstate2)".
+    iInv "Hinv" as "(%state2 & %lstate2 & %ops2 & Hops & Hfd & Hlstate_auth & Hlstate2)".
     wp_load.
     destruct (decide (lstate2 = RcfdLstateOpen)) as [-> | Hlstate2].
 
-    - iDestruct "Hlstate2" as "(%q & %qs & (-> & %Hqs) & (-> & ->) & Htokens_auth & Hmodel)".
+    - iDestruct "Hlstate2" as "(%q & %qs & (-> & %Hqs) & -> & Htokens_auth & Hmodel)".
       iDestruct "H" as "[(%q' & Htokens_frag & Hmodel') | Hlstate_lb]"; last first.
       { iDestruct (rcfd_lstate_valid_closing_no_users with "Hlstate_auth Hlstate_lb") as %?. done. }
       iSplitR "Htokens_frag Hmodel' HΦ". { iExists (RcfdStateOpen _). iSteps. }
@@ -649,7 +647,6 @@ Section rcfd_G.
       iSplitR "H HΦ". { iExists (RcfdStateClosing fn2). iSteps. }
       iModIntro. clear.
 
-      wp_load.
       wp_smart_apply (rcfd_put_spec' with "[$Hinv $H]").
       iSteps. iApply ("HΦ" $! None). iSteps.
   Qed.
@@ -676,11 +673,11 @@ Section rcfd_G.
     wp_rec. wp_pures.
 
     wp_bind (!_)%E.
-    iInv "Hinv" as "(%state1 & %lstate1 & %ops1 & %l_state1 & Hops & Hfd & #Hstate1 & Hlstate_auth & Hlstate1)".
+    iInv "Hinv" as "(%state1 & %lstate1 & %ops1 & Hops & Hfd & Hlstate_auth & Hlstate1)".
     wp_load.
     destruct (decide (lstate1 = RcfdLstateOpen)) as [-> | Hlstate1].
 
-    - iDestruct "Hlstate1" as "(%q & %qs & (-> & %Hqs) & (-> & ->) & Htokens_auth & Hmodel)".
+    - iDestruct "Hlstate1" as "(%q & %qs & (-> & %Hqs) & -> & Htokens_auth & Hmodel)".
       destruct closing; last iClear "Hclosing".
       { iDestruct "Hclosing" as "(%_l & %_γ & %Heq & _Hmeta & Hlstate_lb)". injection Heq as <-.
         iDestruct (meta_agree with "Hmeta _Hmeta") as %<-. iClear "_Hmeta".
@@ -689,16 +686,17 @@ Section rcfd_G.
       iSplitR "HΦ". { iExists (RcfdStateOpen _). iSteps. }
       iModIntro. clear.
 
-      wp_load.
-      wp_alloc l_state as "Hstate". iMod (pointsto_persist with "Hstate") as "#Hstate".
       wp_pures.
 
       wp_bind (Cas _ _ _).
-      iInv "Hinv" as "(%state2 & %lstate2 & %ops2 & %l_state2 & Hops & Hfd & #Hstate2 & Hlstate_auth & Hlstate2)".
-      wp_cas as Hcas | [= <-].
+      iInv "Hinv" as "(%state2 & %lstate2 & %ops2 & Hops & Hfd & Hlstate_auth & Hlstate2)".
+      wp_cas as Hcas | Hcas Hconsistency.
 
       + iAssert (⌜∃ fn2, state2 = RcfdStateClosing fn2⌝ ∗ rcfd_lstate_lb γ RcfdLstateClosingUsers)%I as "((%fn2 & ->) & #Hlstate_lb)".
         { destruct lstate2; iDecompose "Hlstate2".
+          - iDestruct (rcfd_lstate_lb_get with "Hlstate_auth") as "Hlstate_lb".
+            iDestruct (rcfd_lstate_lb_mono with "Hlstate_lb") as "$"; first done.
+            iSteps.
           - iDestruct (rcfd_lstate_lb_get with "Hlstate_auth") as "$".
             iSteps.
           - iDestruct (rcfd_lstate_lb_get with "Hlstate_auth") as "Hlstate_lb".
@@ -708,7 +706,7 @@ Section rcfd_G.
         iSplitR "HΦ". { iExists (RcfdStateClosing _). iSteps. }
         iSteps.
 
-      + iDestruct (pointsto_agree with "Hstate1 Hstate2") as %[= <-]%(inj _).
+      + destruct state2; last naive_solver. destruct Hconsistency as (_ & [= ->]).
         destruct (decide (lstate2 = RcfdLstateOpen)) as [-> | Hlstate2]; last first.
         { destruct lstate2; iDecompose "Hlstate2"; iSteps. }
         iDestruct "Hlstate2" as "(%q & %qs & (-> & %Hqs) & _ & Htokens_auth & Hmodel)".
@@ -731,27 +729,25 @@ Section rcfd_G.
         wp_pures.
 
         wp_bind (!_)%E.
-        iInv "Hinv" as "(%state3 & %lstate3 & %ops3 & %l_state3 & Hops & Hfd & #Hstate3 & Hlstate_auth & Hlstate3)".
+        iInv "Hinv" as "(%state3 & %lstate3 & %ops3 & Hops & Hfd & Hlstate_auth & Hlstate3)".
         wp_load.
         destruct (decide (ops3 = 0)) as [-> | Hops3]; last iSteps.
         iDestruct (rcfd_lstate_valid_closing_users with "Hlstate_auth Hlstate_lb") as %[-> | ->].
         { iDestruct "Hlstate3" as "(%q & %qs & %fn3 & (% & % & _) & _)". lia. }
         iDestruct "Hlstate3" as "(%fn3 & -> & Hfn3)".
         iRename "Hlstate_lb" into "Hlstate_lb'". iDestruct (rcfd_lstate_lb_get with "Hlstate_auth") as "#Hlstate_lb".
-        iSplitR "HΦ". { iExists (RcfdStateClosing _). iStep 5. done. }
+        iSplitR "HΦ". { iExists (RcfdStateClosing _). iStep 4. done. }
         iModIntro. clear.
 
         wp_pures.
 
-        wp_rec. wp_alloc closed as "Hclosed". wp_pures.
-
         wp_bind (Cas _ _ _).
-        iInv "Hinv" as "(%state4 & %lstate4 & %ops4 & %l_state4 & Hops & Hfd & #Hstate4 & Hlstate_auth & Hlstate4)".
-        wp_cas as Hcas | [= <-]; first iSteps.
+        iInv "Hinv" as "(%state4 & %lstate4 & %ops4 & Hops & Hfd & Hlstate_auth & Hlstate4)".
+        wp_cas as Hcas | Hcas _; first iSteps.
 
         iDestruct (rcfd_lstate_valid_closing_no_users with "Hlstate_auth Hlstate_lb") as %->.
         iDestruct "Hlstate4" as "(%fn4 & -> & Hfn4)".
-        iDestruct (pointsto_agree with "Hstate Hstate4") as %[=<-].
+        destruct Hcas as (_ & [= ->]).
         iSplitR "Hfn4 HΦ". { iExists (RcfdStateClosing _). iSteps. }
         iModIntro. clear.
 
@@ -827,11 +823,11 @@ Section rcfd_G.
     wp_rec. wp_pures.
 
     wp_bind (!_)%E.
-    iInv "Hinv" as "(%state1 & %lstate1 & %ops1 & %l_state1 & Hops & Hfd & #Hstate1 & Hlstate_auth & Hlstate1)".
+    iInv "Hinv" as "(%state1 & %lstate1 & %ops1 & Hops & Hfd & Hlstate_auth & Hlstate1)".
     wp_load.
     destruct (decide (lstate1 = RcfdLstateOpen)) as [-> | Hlstate1].
 
-    - iDestruct "Hlstate1" as "(%q & %qs & (-> & %Hqs) & (-> & ->) & Htokens_auth & Hmodel)".
+    - iDestruct "Hlstate1" as "(%q & %qs & (-> & %Hqs) & -> & Htokens_auth & Hmodel)".
       destruct closing; last iClear "Hclosing".
       { iDestruct "Hclosing" as "(%_l & %_γ & %Heq & _Hmeta & Hlstate_lb)". injection Heq as <-.
         iDestruct (meta_agree with "Hmeta _Hmeta") as %<-. iClear "_Hmeta".
@@ -840,18 +836,19 @@ Section rcfd_G.
       iSplitR "HΦ". { iExists (RcfdStateOpen _). iSteps. }
       iModIntro. clear.
 
-      wp_load.
       wp_alloc flag as "Hflag".
       wp_smart_apply (spsc_latch1_create_spec (unix_fd_model fd (DfracOwn 1) chars) with "[//]") as "%chan (#Hchan_inv & Hchan_producer & Hchan_consumer)".
-      wp_alloc l_state as "Hstate". iMod (pointsto_persist with "Hstate") as "#Hstate".
       wp_pures.
 
       wp_bind (Cas _ _ _).
-      iInv "Hinv" as "(%state2 & %lstate2 & %ops2 & %l_state2 & Hops & Hfd & #Hstate2 & Hlstate_auth & Hlstate2)".
-      wp_cas as Hcas | [= <-].
+      iInv "Hinv" as "(%state2 & %lstate2 & %ops2 & Hops & Hfd & Hlstate_auth & Hlstate2)".
+      wp_cas as Hcas | Hcas Hconsistency.
 
       + iAssert (⌜∃ fn2, state2 = RcfdStateClosing fn2⌝ ∗ rcfd_lstate_lb γ RcfdLstateClosingUsers)%I as "((%fn2 & ->) & #Hlstate_lb)".
         { destruct lstate2; iDecompose "Hlstate2".
+          - iDestruct (rcfd_lstate_lb_get with "Hlstate_auth") as "Hlstate_lb".
+            iDestruct (rcfd_lstate_lb_mono with "Hlstate_lb") as "$"; first done.
+            iSteps.
           - iDestruct (rcfd_lstate_lb_get with "Hlstate_auth") as "$".
             iSteps.
           - iDestruct (rcfd_lstate_lb_get with "Hlstate_auth") as "Hlstate_lb".
@@ -861,7 +858,7 @@ Section rcfd_G.
         iSplitR "HΦ". { iExists (RcfdStateClosing _). iSteps. }
         iSteps. iApply ("HΦ" $! None). iSteps.
 
-      + iDestruct (pointsto_agree with "Hstate1 Hstate2") as %[= <-]%(inj _).
+      + destruct state2; last naive_solver. destruct Hconsistency as (_ & [= ->]).
         destruct (decide (lstate2 = RcfdLstateOpen)) as [-> | Hlstate2]; last first.
         { destruct lstate2; iDecompose "Hlstate2"; iSteps. }
         iDestruct "Hlstate2" as "(%q & %qs & (-> & %Hqs) & _ & Htokens_auth & Hmodel)".
@@ -872,10 +869,10 @@ Section rcfd_G.
           - apply gmultiset_size_empty_iff in Hqs_size as ->.
             rewrite gmultiset_set_fold_empty in Hqs. rewrite {}Hqs.
             iMod (rcfd_lstate_update RcfdLstateClosingNoUsers with "Hlstate_auth") as "Hlstate_auth"; first done.
-            iExists (RcfdStateClosing _). iStep 9. iModIntro.
+            iExists (RcfdStateClosing _). iStep 8. iModIntro.
             wp_apply (spsc_latch1_signal_spec with "[$Hchan_inv $Hchan_producer $Hmodel]").
             iSteps.
-          - iExists (RcfdStateClosing _). iStep 11 as "Hmodel". iModIntro.
+          - iExists (RcfdStateClosing _). iStep 10 as "Hmodel". iModIntro.
             wp_apply (spsc_latch1_signal_spec with "[$Hchan_inv $Hchan_producer $Hmodel]").
             iSteps.
         }
@@ -988,7 +985,7 @@ Section rcfd_G.
     wp_rec. wp_pures.
 
     wp_bind (!#l.[fd])%E.
-    iInv "Hinv" as "(%state & %lstate & %ops & %l_state & Hops & Hfd & #Hstate & Hlstate_auth & Hlstate)".
+    iInv "Hinv" as "(%state & %lstate & %ops & Hops & Hfd & Hlstate_auth & Hlstate)".
     wp_load.
     destruct closing; last iClear "Hclosing".
 
@@ -1074,7 +1071,7 @@ Section rcfd_G.
     wp_rec. wp_pures.
 
     wp_bind (!#l.[fd])%E.
-    iInv "Hinv" as "(%state & %lstate & %ops & %l_state & Hops & Hfd & #Hstate & Hlstate_auth & Hlstate)".
+    iInv "Hinv" as "(%state & %lstate & %ops & Hops & Hfd & Hlstate_auth & Hlstate)".
     wp_load.
     destruct closing; last iClear "Hclosing".
 
