theories/language/syntax.v
@@ -23,6 +23,10 @@ Definition prophecy_id :=
   positive.
 Implicit Types p : prophecy_id.
 
+Definition constr_id :=
+  positive.
+Implicit Types cid : option constr_id.
+
 Inductive literal :=
   | LiteralBool b
   | LiteralInt n
@@ -173,6 +177,7 @@ Inductive expr :=
   | Constr tag (es : list expr)
   | Proj proj (e : expr)
   | Match (e0 : expr) x (e1 : expr) (brs : list (pattern * expr))
+  | Reveal (e : expr)
   | For (e1 e2 e3 : expr)
   | Record (es : list expr)
   | Alloc (e1 e2 : expr)
@@ -187,7 +192,7 @@ Inductive expr :=
 with val :=
   | ValLiteral lit
   | ValRec f x (e : expr)
-  | ValConstr tag (vs : list val).
+  | ValConstr cid tag (vs : list val).
 Set Elimination Schemes.
 Implicit Types e : expr.
 Implicit Types es : list expr.
@@ -209,9 +214,9 @@ Section val_ind.
     ∀ f x e,
     P (ValRec f x e).
   Variable HValConstr :
-    ∀ tag,
+    ∀ cid tag,
     ∀ vs, Forall P vs →
-    P (ValConstr tag vs).
+    P (ValConstr cid tag vs).
 
   Fixpoint val_ind v :=
     match v with
@@ -219,8 +224,8 @@ Section val_ind.
         HValLiteral lit
     | ValRec f x e =>
         HValRec f x e
-    | ValConstr tag vs =>
-        HValConstr tag
+    | ValConstr cid tag vs =>
+        HValConstr cid tag
           vs (Forall_true P vs val_ind)
     end.
 End val_ind.
@@ -274,6 +279,9 @@ Section expr_ind.
     ∀ e1, P e1 →
     ∀ brs, Forall (λ br, P br.2) brs →
     P (Match e0 x e1 brs).
+  Variable HReveal :
+    ∀ e, P e →
+    P (Reveal e).
   Variable HFor :
     ∀ e1, P e1 →
     ∀ e2, P e2 →
@@ -358,6 +366,9 @@ Section expr_ind.
           x
           e1 (expr_ind e1)
           brs (Forall_true (λ br, P br.2) brs (λ br, expr_ind br.2))
+    | Reveal e =>
+        HReveal
+          e (expr_ind e)
     | For e1 e2 e3 =>
         HFor
           e1 (expr_ind e1)
@@ -426,11 +437,11 @@ Notation ValProphecy p := (
 ).
 
 Notation Tuple := (
-  Constr 0
+  Constr None 0
 )(only parsing
 ).
 Notation ValTuple := (
-  ValConstr 0
+  ValConstr None 0
 )(only parsing
 ).
 
@@ -615,6 +626,9 @@ Proof.
             (decide (x1 = x2))
             (decide (e11 = e21))
             (decide (brs1 = brs2))
+      | Reveal e1, Reveal e2 =>
+          cast_if
+            (decide (e1 = e2))
       | For e11 e12 e13, For e21 e22 e23 =>
           cast_if_and3
             (decide (e11 = e21))
@@ -682,8 +696,9 @@ Proof.
             (decide (f1 = f2))
             (decide (x1 = x2))
             (decide (e1 = e2))
-      | ValConstr tag1 es1, ValConstr tag2 es2 =>
-          cast_if_and
+      | ValConstr cid1 tag1 es1, ValConstr cid2 tag2 es2 =>
+          cast_if_and3
+            (decide (cid1 = cid2))
             (decide (tag1 = tag2))
             (decide (es1 = es2))
       | _, _ =>
@@ -719,8 +734,9 @@ Proof.
             (decide (f1 = f2))
             (decide (x1 = x2))
             (decide (e1 = e2))
-      | ValConstr tag1 es1, ValConstr tag2 es2 =>
-          cast_if_and
+      | ValConstr cid1 tag1 es1, ValConstr cid2 tag2 es2 =>
+          cast_if_and3
+            (decide (cid1 = cid2))
             (decide (tag1 = tag2))
             (decide (es1 = es2))
       | _, _ =>
@@ -734,6 +750,7 @@ Variant encode_leaf :=
   | EncodeUnop (op : unop)
   | EncodeBinop (op : binop)
   | EncodeProjection proj
+  | EncodeConstrId cid
   | EncodeConstrTag tag
   | EncodePattern (pat : pattern)
   | EncodeLiteral lit.
@@ -745,13 +762,15 @@ Proof.
   pose encode leaf :=
     match leaf with
     | EncodeBinder x =>
-        inl $ inl $ inl $ inl $ inl $ inl x
+        inl $ inl $ inl $ inl $ inl $ inl $ inl x
     | EncodeUnop op =>
-        inl $ inl $ inl $ inl $ inl $ inr op
+        inl $ inl $ inl $ inl $ inl $ inl $ inr op
     | EncodeBinop op =>
-        inl $ inl $ inl $ inl $ inr op
+        inl $ inl $ inl $ inl $ inl $ inr op
     | EncodeProjection proj =>
-        inl $ inl $ inl $ inr proj
+        inl $ inl $ inl $ inl $ inr proj
+    | EncodeConstrId cid =>
+        inl $ inl $ inl $ inr cid
     | EncodeConstrTag tag =>
         inl $ inl $ inr tag
     | EncodePattern pat =>
@@ -761,14 +780,16 @@ Proof.
     end.
   pose decode leaf :=
     match leaf with
-    | inl (inl (inl (inl (inl (inl x))))) =>
+    | inl (inl (inl (inl (inl (inl (inl x)))))) =>
         EncodeBinder x
-    | inl (inl (inl (inl (inl (inr op))))) =>
+    | inl (inl (inl (inl (inl (inl (inr op)))))) =>
         EncodeUnop op
-    | inl (inl (inl (inl (inr op)))) =>
+    | inl (inl (inl (inl (inl (inr op))))) =>
         EncodeBinop op
-    | inl (inl (inl (inr proj))) =>
+    | inl (inl (inl (inl (inr proj)))) =>
         EncodeProjection proj
+    | inl (inl (inl (inr cid))) =>
+        EncodeConstrId cid
     | inl (inl (inr tag)) =>
         EncodeConstrTag tag
     | inl (inr pat) =>
@@ -804,30 +825,32 @@ Proof.
     8.
   Notation code_Match :=
     9.
-  Notation code_For :=
+  Notation code_Reveal :=
     10.
-  Notation code_branch :=
+  Notation code_For :=
     11.
-  Notation code_Record :=
+  Notation code_branch :=
     12.
-  Notation code_Alloc :=
+  Notation code_Record :=
     13.
-  Notation code_Load :=
+  Notation code_Alloc :=
     14.
-  Notation code_Store :=
+  Notation code_Load :=
     15.
-  Notation code_Xchg :=
+  Notation code_Store :=
     16.
-  Notation code_Cas :=
+  Notation code_Xchg :=
     17.
-  Notation code_Faa :=
+  Notation code_Cas :=
     18.
-  Notation code_Fork :=
+  Notation code_Faa :=
     19.
-  Notation code_Proph :=
+  Notation code_Fork :=
     20.
-  Notation code_Resolve :=
+  Notation code_Proph :=
     21.
+  Notation code_Resolve :=
+    22.
   Notation code_ValRec :=
     0.
   Notation code_ValConstr :=
@@ -862,6 +885,8 @@ Proof.
           GenNode code_Proj [GenLeaf (EncodeProjection proj); go e]
       | Match e0 x e1 brs =>
           GenNode code_Match $ go e0 :: GenLeaf (EncodeBinder x) :: go e1 :: go_branches brs
+      | Reveal e =>
+          GenNode code_Reveal [go e]
       | For e1 e2 e3 =>
           GenNode code_For [go e1; go e2; go e3]
       | Record es =>
@@ -892,8 +917,8 @@ Proof.
           GenLeaf (EncodeLiteral lit)
       | ValRec f x e =>
          GenNode code_ValRec [GenLeaf (EncodeBinder f); GenLeaf (EncodeBinder x); go e]
-      | ValConstr tag vs =>
-          GenNode code_ValConstr $ GenLeaf (EncodeConstrTag tag) :: go_list vs
+      | ValConstr cid tag vs =>
+          GenNode code_ValConstr $ GenLeaf (EncodeConstrId cid) :: GenLeaf (EncodeConstrTag tag) :: go_list vs
       end
     for go.
   pose decode :=
@@ -931,6 +956,8 @@ Proof.
           Proj proj $ go e
       | GenNode code_Match (e0 :: GenLeaf (EncodeBinder x) :: e1 :: brs) =>
           Match (go e0) x (go e1) (go_branches brs)
+      | GenNode code_Reveal [e] =>
+          Reveal (go e)
       | GenNode code_For [e1; e2; e3] =>
           For (go e1) (go e2) (go e3)
       | GenNode code_Record es =>
@@ -963,8 +990,8 @@ Proof.
           ValLiteral lit
       | GenNode code_ValRec [GenLeaf (EncodeBinder f); GenLeaf (EncodeBinder x); e] =>
           ValRec f x (go e)
-      | GenNode code_ValConstr (GenLeaf (EncodeConstrTag tag) :: vs) =>
-          ValConstr tag $ go_list vs
+      | GenNode code_ValConstr (GenLeaf (EncodeConstrId cid) :: GenLeaf (EncodeConstrTag tag) :: vs) =>
+          ValConstr cid tag $ go_list vs
       | _ =>
           @inhabitant _ val_inhabited
       end
