theories/saturn/bag.v
@@ -257,7 +257,7 @@ Section bag_G.
     iDestruct (big_sepL2_length with "Hslots") as "#>%Hlen".
     destruct (lookup_lt_is_Some_2 os i) as (o & Hos_lookup); first congruence.
     iDestruct (big_sepL2_insert_acc with "Hslots") as "(Hslot & Hslots)"; [done.. |].
-    wp_cas as _ | ->%(inj opt_to_val _ None).
+    wp_cas as _ | ->%(inj opt_to_val _ None) _.
 
     - iDestruct ("Hslots" with "Hslot") as "Hslots".
       rewrite !list_insert_id //.
@@ -352,7 +352,7 @@ Section bag_G.
     iDestruct (big_sepL2_length with "Hslots") as "#>%Hlen".
     destruct (lookup_lt_is_Some_2 os i) as (o & Hos_lookup); first congruence.
     iDestruct (big_sepL2_insert_acc with "Hslots") as "(Hslot & Hslots)"; [done.. |].
-    wp_cas as _ | ->%(inj opt_to_val _ (Some v)).
+    wp_cas as _ | ->%(inj opt_to_val _ (Some v)) _.
 
     - iDestruct ("Hslots" with "Hslot") as "Hslots".
       rewrite !list_insert_id //.
