theories/saturn/mpmc_stack.v
@@ -144,7 +144,7 @@ Section zebre_G.
 
     wp_bind (Cas _ _ _).
     iInv "Hinv" as "(%vs' & Hl & Hmodel₂)".
-    wp_cas as _ | ->%(inj _); first iSteps.
+    wp_cas as _ | ->%(inj _) _; first iSteps.
     iMod "HΦ" as "(%_vs & (%_l & %_γ & %Heq & _Hmeta & Hmodel₁) & _ & HΦ)". injection Heq as <-.
     iDestruct (meta_agree with "Hmeta _Hmeta") as %<-. iClear "_Hmeta".
     iDestruct (twins_agree_L with "Hmodel₁ Hmodel₂") as %->.
@@ -190,7 +190,7 @@ Section zebre_G.
 
       wp_bind (Cas _ _ _).
       iInv "Hinv" as "(%vs' & Hl & Hmodel₂)".
-      wp_cas as _ | Hcas; first iSteps.
+      wp_cas as _ | Hcas _; first iSteps.
       destruct vs'; first done. apply (inj lst_to_val _ (_ :: _)) in Hcas as [= -> ->].
       iMod "HΦ" as "(%_vs & (%_l & %_γ & %Heq & _Hmeta & Hmodel₁) & _ & HΦ)". injection Heq as <-.
       iDestruct (meta_agree with "Hmeta _Hmeta") as %<-. iClear "_Hmeta".
