theories/std/queue.v
@@ -98,7 +98,7 @@ Section zebre_G.
     destruct vs as [| v vs].
     - iDestruct (chain_model_nil with "Hfront_model") as %->.
       iDestruct (chain_physical with "Hsent_model") as %Hphysical; first naive_solver.
-      wp_equal as ? | _.
+      wp_equal as ? | _ _.
       { iDestruct (chain_physically_distinct' with "Hsent_model") as %[]; naive_solver. }
       iSteps.
     - wp_apply (wp_equal_chain with "Hfront_model Hsent_model") as "Hfront_model Hsent_model"; [naive_solver lia.. |].
